Attempt to write a first version of progress_pure

backends/lean/Aeneas/Progress/Core.lean
@@ -2,6 +2,7 @@ import Lean
 import Aeneas.Utils
 import Aeneas.Std.Core
 import Aeneas.Extensions
+import Aeneas.Progress.Trace
 
 namespace Aeneas
 
@@ -9,9 +10,6 @@ namespace Progress
 
 open Lean Elab Term Meta
 open Utils Extensions
-
--- We can't define and use trace classes in the same file
-initialize registerTraceClass `Progress
 
 /- # Progress tactic -/
 
@@ -104,7 +102,7 @@ section Methods
       -- If we are registering a theorem, then the function must be a constant
       if ¬ f.isConst then
         if isGoal then pure []
-        else throwError "Not a constant: {f}"
+        else throwError "{f} should be a constant"
       else pure f.constLevels!
     -- *Sanity check* (activated if we are analyzing a theorem to register it in a DB)
     -- Check if some existentially quantified variables
@@ -131,48 +129,51 @@ section Methods
       post := post
     }
     k thDesc
-
 end Methods
 
 def getPSpecFunArgsExpr (isGoal : Bool) (th : Expr) : MetaM Expr :=
   withPSpec isGoal th (fun d => do pure d.fArgsExpr)
 
--- pspec attribute
+-- The progress attribute
 structure PSpecAttr where
   attr : AttributeImpl
   ext  : DiscrTreeExtension Name
   deriving Inhabited
 
-/- The persistent map from expressions to pspec theorems. -/
+private def saveProgressSpecFromThm (ext : DiscrTreeExtension Name) (attrKind : AttributeKind) (thName : Name) :
+  AttrM Unit := do
+  -- TODO: use the attribute kind
+  unless attrKind == AttributeKind.global do
+    throwError "invalid attribute 'progress', must be global"
+  -- Lookup the theorem
+  let env ← getEnv
+  -- Ignore some auxiliary definitions (see the comments for attrIgnoreMutRec)
+  attrIgnoreAuxDef thName (pure ()) do
+    trace[Progress] "Registering `progress` theorem for {thName}"
+    let thDecl := env.constants.find! thName
+    let fKey ← MetaM.run' (do
+      trace[Progress] "Theorem: {thDecl.type}"
+      -- Normalize to eliminate the let-bindings
+      let ty ← normalizeLetBindings thDecl.type
+      trace[Progress] "Theorem after normalization (to eliminate the let bindings): {ty}"
+      let fExpr ← getPSpecFunArgsExpr false ty
+      trace[Progress] "Registering spec theorem for expr: {fExpr}"
+      -- Convert the function expression to a discrimination tree key
+      DiscrTree.mkPath fExpr)
+    let env := ext.addEntry env (fKey, thName)
+    setEnv env
+    trace[Progress] "Saved the environment"
+    pure ()
+
+/- Initiliaze the `progress` attribute. -/
 initialize pspecAttr : PSpecAttr ← do
   let ext ← mkDiscrTreeExtension `pspecMap
   let attrImpl : AttributeImpl := {
     name := `progress
-    descr := "Marks theorems to use with the `progress` tactic"
+    descr := "Adds theorems to the `progress` database"
     add := fun thName stx attrKind => do
       Attribute.Builtin.ensureNoArgs stx
-      -- TODO: use the attribute kind
-      unless attrKind == AttributeKind.global do
-        throwError "invalid attribute 'pspec', must be global"
-      -- Lookup the theorem
-      let env ← getEnv
-      -- Ignore some auxiliary definitions (see the comments for attrIgnoreMutRec)
-      attrIgnoreAuxDef thName (pure ()) do
-        trace[Progress] "Registering spec theorem for {thName}"
-        let thDecl := env.constants.find! thName
-        let fKey ← MetaM.run' (do
-          trace[Progress] "Theorem: {thDecl.type}"
-          -- Normalize to eliminate the let-bindings
-          let ty ← normalizeLetBindings thDecl.type
-          trace[Progress] "Theorem after normalization (to eliminate the let bindings): {ty}"
-          let fExpr ← getPSpecFunArgsExpr false ty
-          trace[Progress] "Registering spec theorem for expr: {fExpr}"
-          -- Convert the function expression to a discrimination tree key
-          DiscrTree.mkPath fExpr)
-        let env := ext.addEntry env (fKey, thName)
-        setEnv env
-        trace[Progress] "Saved the environment"
-        pure ()
+      saveProgressSpecFromThm ext attrKind thName
   }
   registerBuiltinAttribute attrImpl
   pure { attr := attrImpl, ext := ext }
@@ -190,6 +191,307 @@ def showStoredPSpec : MetaM Unit := do
   let s := f!"{st}"
   IO.println s
 
+/-- Convert a list of fvars to a structure. TODO: for now we just create a big tuple, and it may not always work... -/
+private def fvarsToStruct (fvars : Array Expr) : MetaM Expr := do
+  mkProdsVal fvars.toList
+
+private def mkExistsFVars (fvars : Array Expr) (body : Expr) : MetaM Expr := do
+  let rec aux (fvars : List Expr) : MetaM Expr :=
+    match fvars with
+    | [] => pure body
+    | fv :: fvars => do
+      let e ← aux fvars
+      let thm ← mkLambdaFVars #[fv] e
+      mkAppM ``Exists #[thm]
+  aux fvars.toList
+
+/-- Auxiliary helper for `progress_pure` -/
+private def liftThm (thm : Expr) : MetaM Expr := do
+  forallTelescope thm fun fvars thm => do
+  match thm with
+  | .letE (declName : Name) declTy (value : Expr) (post : Expr) _ => do
+    /- Introduce an fvar for the local declaration -/
+    withLocalDeclD declName declTy fun fv => do
+    /- Create the lifted expression -/
+    let bound ← mkAppM ``Std.toResult #[value]
+    let okExpr ← mkAppM ``Std.Result.ok #[fv]
+    let eq ← mkAppM ``Eq #[bound, okExpr]
+    /- Introduce the existential -/
+    let thm ← mkLambdaFVars #[fv] (mkAnd eq post)
+    let thm ← mkAppM ``Exists #[thm]
+    /- Introduce the foralls -/
+    mkLambdaFVars fvars thm
+  | _ => do
+    /- "Complex" let-bindings such as `let (x, y) := ...` are actually desugared to matches -/
+    let me ← matchMatcherApp? thm
+    let error (_ : Unit) : MetaM Expr := do throwError "The theorem does not have the proper shape: the statement after the universally quantified variables should start with a let-binding; found {thm} instead."
+    let .some me := me
+      | error ()
+    if me.alts.size ≠ 1 ∨ me.discrs.size ≠ 1 then error ()
+    else
+    let numParams := me.altNumParams[0]!
+    let branch := me.alts[0]!
+    let discr := me.discrs[0]!
+    /- Destruct the universally quantified variables -/
+    forallTelescope branch.consumeMData fun fvars' post => do
+    let fvars'' := fvars'.extract numParams fvars'.size
+    let fvars' := fvars'.extract 0 numParams
+    let post ← mkLambdaFVars fvars'' post
+    /- Create the lifted expression -/
+    let bound ← mkAppM ``Std.toResult #[discr]
+    let okExpr ← mkAppM ``Std.Result.ok #[← fvarsToStruct fvars']
+    let eq ← mkAppM ``Eq #[bound, okExpr]
+    /- Introduce the existentials -/
+    let thm ← mkExistsFVars fvars' (mkAnd eq post)
+    /- Introduce the foralls -/
+    mkLambdaFVars fvars thm
+
+open Tactic
+
+#check @Eq
+
+namespace Test
+  /-!
+  Making some tests here to see how we should generate the proof terms when lifting theorems in `progress_pure`
+  -/
+  open Std Result
+  def mk_pos_pair : Int × Int := (0, 1)
+
+  theorem is_pos :
+    let (x, y) := mk_pos_pair
+    x ≥ 0 ∧ y ≥ 0 := by simp [mk_pos_pair]
+
+  theorem lifted_is_pos :
+    ∃ x y, toResult mk_pos_pair = ok (x, y) ∧
+    x ≥ 0 ∧ y ≥ 0 :=
+  (match mk_pos_pair with
+  | (x, y) =>
+    fun (h : match (x, y) with | (x, y) => x ≥ 0 ∧ y ≥ 0) =>
+    Exists.intro x (Exists.intro y (And.intro (Eq.refl (ok (x, y))) h))
+  : ∀ (_ : match mk_pos_pair with | (x, y) => x ≥ 0 ∧ y ≥ 0),
+    ∃ x y, toResult mk_pos_pair = ok (x, y) ∧
+    x ≥ 0 ∧ y ≥ 0) is_pos
+
+
+  set_option pp.coercions false
+  set_option pp.all false
+  set_option pp.explicit true
+  #print lifted_is_pos
+end Test
+
+partial def destProdTy (x : Expr) : List Expr :=
+  x.consumeMData.withApp fun f args =>
+  if f.isConst ∧ f.constName = ``Prod ∧ args.size = 2 then
+    let ty0 := args[0]!
+    let ty1 := args[1]!
+    ty0 :: destProdTy ty1
+  else [x]
+
+partial def destProdVal (x : Expr) : List Expr :=
+  x.consumeMData.withApp fun f args =>
+  if f.isConst ∧ f.constName = ``Prod.mk ∧ args.size = 4 then
+    let val0 := args[2]!
+    let val1 := args[3]!
+    val0 :: destProdVal val1
+  else [x]
+
+
+#check mkFreshFVarId
+#check @Exists.intro
+#check Declaration
+#check mkArrowN
+def tryGeneralize (pat : Syntax) (n : Name) : TermElabM Unit := do
+  trace[Progress] "Name: {n}"
+  let env ← getEnv
+  let decl := env.constants.find! n
+  -- Strip the quantifiers before elaborating the pattern
+  forallTelescope decl.type.consumeMData fun fvars thm0 => do
+  let (pat, _) ← Elab.Term.elabTerm pat none |>.run
+  trace[Progress] "Elaborated pattern: {pat}"
+  --
+  existsTelescope pat.consumeMData fun fvarsPat eq => do
+  /- Destruct the equality. Note that there may not be a tuple, in which case
+     we introduce a single variable -/
+  let tryDestEq (k : Expr → Expr → TermElabM Unit) : TermElabM Unit := do
+    match ← destEqOpt eq with
+    | some (x, y) => k x y
+    | none =>
+      let pat := eq
+      let ty ← inferType pat
+      let name ← mkFreshUserName (.str .anonymous "x")
+      withLocalDeclD name ty fun decompPat => do
+      k pat decompPat
+  tryDestEq fun pat decompPat => do
+  trace[Progress] "Decomposed equality: {pat}, {decompPat}"
+  -- The decomp pattern should be a tuple
+  let pats := destProdVal decompPat
+  trace[Progress] "Decomposed pattern: {pats}"
+  -- Update the theorem statement to replace the pattern with the decomposed pattern
+  let thm1 ←
+    mapVisit (fun _ e => do if e == pat then pure decompPat else pure e) thm0
+  trace[Progress] "Updated theorem statement: {thm1}"
+  -- Dive into the λ which binds the pure theorem
+  let pureThmName ← mkFreshUserName (.str .anonymous "pureThm")
+  withLocalDeclD pureThmName thm1 fun pureThm => do
+  -- Introduce the equality
+  let okDecompPat ← mkAppM ``Std.Result.ok #[decompPat]
+  let toResultPat ← mkAppM ``Std.toResult #[pat]
+  let eqExpr ← mkAppM ``Eq.refl #[okDecompPat]
+  /-let eqType ← mkAppM ``Eq #[toResultPat, okDecompPat]
+  let thm ← mkAppOptM ``And.intro #[eqType, none, eqExpr, pureThm]-/
+  let thm ← mkAppOptM ``And.intro #[none, none, eqExpr, pureThm]
+  trace[Progress] "Theorem after introducing the lifted equality: {thm} : {← inferType thm}"
+  -- Introduce the existentials
+  let thm ←
+    Array.foldrM (fun fvar thm => do
+      let p ← mkLambdaFVars #[fvar] (← inferType thm)
+      mkAppOptM ``Exists.intro #[← inferType fvar, p, fvar, thm]
+      ) thm fvarsPat
+  trace[Progress] "Theorem after introducing the existentials: {thm} :\n{← inferType thm}"
+  -- Introduce the λ which binds the pure theorem
+  let thm ← mkLambdaFVars #[pureThm] thm
+  trace[Progress] "Theorem after introducing the lambda: {thm} :\n{← inferType thm}"
+  -- Introduce the matches
+  let thm ← mkProdsMatch pats thm -- TODO: should be mkProdsMatch
+  let thm ← mkAppM' thm #[pat]
+  trace[Progress] "Theorem after introducing the matches: {thm} :\n{← inferType thm}"
+  -- Apply the pure theorem
+  let thm := mkAppN thm #[.const decl.name (List.map Level.param decl.levelParams)]
+  let thm ← mkLambdaFVars fvars thm
+  trace[Progress] "Final theorem: {thm} :\n{← inferType thm}"
+  -- Prepare the type of the final theorem
+  let thmType := thm1
+  trace[Progress] "Theorem type without lifted equality: {thmType}"
+  let eqType ← mkEq toResultPat okDecompPat
+  trace[Progress] "Theorem type after lifting equality: {thmType}"
+  let thmType := mkAnd eqType thmType
+  -- Introduce the existentials
+  let thmType ← Array.foldrM (fun fvar thmType => do
+      let p ← mkLambdaFVars #[fvar] thmType
+      mkAppOptM ``Exists #[← inferType fvar, p]
+      ) thmType fvarsPat
+  trace[Progress] "Theorem type: {thmType}"
+  --let pureThmType ← mkArrowN fvars (← inferType existsThm)
+  -- Save the auxiliary theorem
+  let auxDecl : TheoremVal := {
+    name := Name.str decl.name "progress_spec"
+    levelParams := decl.levelParams
+    type := thmType
+    value := thm
+  }
+  addDecl (.thmDecl auxDecl)
+  --
+  --let thm ← mkLambdaFVars #[pureThm] pureThm
+  pure ()
+  /--- Introduce matches
+  let rec introMatches (decompPat : Expr) (k : TermElabM Unit) := do
+    match decompPat with
+    | .
+  pure ()-/
+
+
+local elab "#try_generalize" "(" pat:term ")" id:ident : command => do
+  Lean.Elab.Command.runTermElabM (fun _ => do
+  let some cs ← Term.resolveId? id | throwError m!"Unknown id: {id}"
+  let name := cs.constName!
+  tryGeneralize pat name)
+
+set_option trace.Progress true in
+#try_generalize (∃ x y, Test.mk_pos_pair = (x, y)) Test.is_pos
+
+#check Test.is_pos.progress_spec
+
+/-- Auxiliary helper: prove the auxiliary theorem (generates the proof term) -/
+private def pspecPureProve (pureThm : ConstantInfo) (th : Expr) : TermElabM Expr := do
+  let goal ← mkFreshExprMVar (some th)
+  let prove : TacticM Unit := do
+    let goal ← getMainGoal
+    let (_, goal) ← goal.intros
+    setGoals [goal]
+    let lctx ← getLCtx
+    -- Introduce the lemma
+    let levelParams := List.map Level.param pureThm.levelParams
+    let pureThmExpr := Expr.const pureThm.name levelParams
+    let pureThmExpr := mkAppN pureThmExpr lctx.getFVars
+    let pureThmExprName ← mkFreshUserName (.str .anonymous "auxThm")
+    withLetDecl pureThmExprName (← inferType pureThmExpr) pureThmExpr fun _ => do
+    -- We simply call the simplifier
+    let simpOnly := true
+    let config : Simp.Config := {}
+    let simprocs := []
+    let declsToUnfold := []
+    let thms := []
+    let loc := Utils.Location.targets #[] true
+    let pureThm ← getFVarFromUserName pureThmExprName
+    simpAt simpOnly config simprocs declsToUnfold thms [pureThm.fvarId!] loc
+    let lctx ← getLCtx
+    let hypsToUse := lctx.getFVarIds
+    simpAt simpOnly config simprocs declsToUnfold thms hypsToUse.toList loc
+  let ngoals ← Tactic.run goal.mvarId! prove
+  /- There should be no remaining goals -/
+  if ngoals == [] then
+    pure (← instantiateMVars goal)
+  else
+    throwError "Error while elaborating 'progress_spec': we could not prove the auxiliary theorem"
+
+/- Initiliaze the `progress_pure` attribute, which lifts lemmas about pure functions to
+   `progress` lemmas.
+
+   For instance, if we annotate the following theorem with `progress_pure` (note the `let` binding
+   which must be at the beginning of the theorem statement):
+   ```
+   @[progress_pure]
+   theorem U32.wrapping_add_eq (x y : U32) :
+    let z := wrapping_add x y
+    z.bv = x.bv + y.bv
+   ```
+   `progress_pure` introduces the following intermediate definition:
+   ```
+   @[progress_pure]
+   theorem U32.wrapping_add_eq.progress_spec (x y : U32) :
+    ∃ z, ↑(wrapping_add x y) = ok z ∧
+    z.bv = x.bv + y.bv
+   ```
+ -/
+initialize pspecPureAttribute : PSpecAttr ← do
+  let ext ← mkDiscrTreeExtension `pspecMap
+  let attrImpl : AttributeImpl := {
+    name := `progress_pure
+    descr := "Adds lifted version of pure theorems to the `progress_pure` databse"
+    add := fun thName stx attrKind => do
+      Attribute.Builtin.ensureNoArgs stx
+      -- TODO: use the attribute kind
+      unless attrKind == AttributeKind.global do
+        throwError "invalid attribute 'progress_pure', must be global"
+      -- Lookup the theorem
+      let env ← getEnv
+      -- Ignore some auxiliary definitions (see the comments for attrIgnoreMutRec)
+      attrIgnoreAuxDef thName (pure ()) do
+        trace[Progress] "Registering pure `progress` theorem for {thName}"
+        let thDecl := env.constants.find! thName
+        -- Lift the theorem statement
+        let liftedThm ← MetaM.run' (liftThm thDecl.type.consumeMData)
+        -- Prove the lifted statement
+        let value ← liftM (pspecPureProve thDecl liftedThm)
+        -- Save an auxiliary theorem for the lifted statement
+        let liftedThmName := Name.str thName "progress_spec"
+        let liftedThmDecl := Declaration.defnDecl {
+          name := Name.str thName "progress_spec"
+          levelParams := thDecl.levelParams
+          type := liftedThm
+          value := value
+          hints := .opaque
+          safety := .safe
+          all := [liftedThmName]
+        }
+        addDecl liftedThmDecl
+        -- Save the auxiliary theorem to the `progress` database
+        saveProgressSpecFromThm pspecAttr.ext attrKind liftedThmName
+  }
+  registerBuiltinAttribute attrImpl
+  pure { attr := attrImpl, ext := ext }
+
+#check elabTerminationHints
 end Progress
 
 end Aeneas
